Move [RecordRepr] typeclass out of test and into rules

rocq-osiris/theories/program_logic/rules/record_rules.v
@@ -242,3 +242,93 @@ Section records_reasoning.
   Qed.
 
 End records_reasoning.
+
+(* So far, our logical model of records has been tuples. Although this
+   is sufficiently expressive for most purposes, we can allow users to
+   provide their own logical model by mapping to our tuples. *)
+
+Section encoded_fields.
+
+  Context `{!osirisGS Σ}.
+
+  (* [RecordRepr A τ t] ties a logical model type [A] to a record with
+     fields described by [τ] and with mutable tag [t]. *)
+
+  (* For example, a record type [point := { x : Z; y : Z }] would need
+     an instance [RecordRepr point τ[Z; Z] (Mut/Immut)]. *)
+
+  Class RecordRepr (A : Type) (τ : types) (t : mut_tag) :=
+    { repr_to_types : A → τ;
+      types_to_repr : τ -#> A;
+      repr_id : ∀ xs, (repr_to_types ∘ types_to_repr) xs = xs }.
+
+  (* [ownRepr] defines the ownership of a record with logical model [a : A]. *)
+
+  Definition ownRepr `{RecordRepr A τ t} (r : record) qp (a : A) : iProp Σ :=
+    ownRecord (τ:=τ) r qp t (repr_to_types a).
+
+  Instance ownRepr_fractional `{RecordRepr A τ t} r (a : A) : Fractional (λ qp, ownRepr r qp a) := _.
+
+  Global Instance ownRepr_as_fractional `{RecordRepr A t} (r : record) q (a : A) :
+    AsFractional (ownRepr r q a) (λ q, ownRepr r q a) q.
+  Proof. constructor; done || apply _. Qed.
+
+  (* -------------------------------------------------------------------------- *)
+
+  (* We can now redefine reasoning rules in terms of user-provided
+     logical models, instead of tuples. *)
+
+  Lemma imp_record `{RecordRepr A τ t} {η E Ψ ζ} es (Φs : τ -#> iProp Σ) :
+    (τ_length τ ≤ max_array_length)%Z →
+    impure E (evals η es) Ψ ζ Φs -∗
+    impure E (eval η (ERecord t es)) Ψ ζ (λ r, ∃# (xs : τ), ownRepr r 1 (types_to_repr xs) ∗ Φs xs).
+  Proof.
+    iIntros (Hlength) "Hes".
+    iApply (imp_wand with "[-]").
+    { iApply (imp_ERecord with "Hes"). assumption. }
+    iIntros (r).
+    rewrite !bi_texist_equiv.
+    iIntros "(%xs & Hr & HΦ)".
+    iFrame. unfold ownRepr.
+    pose proof repr_id as Hid. simpl in Hid. rewrite Hid.
+    iApply "Hr".
+  Qed.
+
+  Lemma imp_record_access `{RecordRepr A τ t} {η E Ψ ζ} f (r : record) (qp : Qp) (a : A) (e : expr) :
+    valid_field f τ →
+    ▷ ownRepr r qp a -∗
+    impure E (eval η e) Ψ ζ (λ r', ⌜r' = r⌝) -∗
+    impure E (eval η (ERecordAccess e f)) Ψ ζ (λ (x : τ !!! f), ⌜x = repr_to_types a !!τ f⌝ ∗ ownRepr r qp a).
+  Proof.
+    iIntros (Hvalid) "Hown He".
+    iApply (imp_wand with "[-]").
+    { iApply (imp_ERecordAccess with "Hown He"). assumption. }
+    iIntros (x) "($ & $)".
+  Qed.
+
+  (* Despite what we might expect, we do not require the record to be
+     mutable for an update to occur. The OCaml typechecker should make
+     such a situation impossible, so we only expect this to be relevant
+     in the case where unsafe type coercions were used. In such a case,
+     our semantics allow updating records with "immutable" fields as
+     long as we have full ownership. *)
+
+  Lemma imp_record_update `{RecordRepr A τ t} {η E Ψ ζ} (r : record) f (a : A) e1 e2 Φ :
+    valid_field f τ →
+    ▷ ownRepr r 1 a -∗
+    impure E (eval η e1) Ψ ζ (λ r', ⌜r' = r⌝) -∗
+    impure E (eval η e2) Ψ ζ Φ -∗
+    impure E (eval η (ERecordSet e1 f e2)) Ψ ζ
+      (λ _ : unit, ∃ (x : τ !!! f), Φ x ∗ ownRepr r 1 (types_to_repr (<[ f τ= x]> (repr_to_types a)))).
+  Proof.
+    iIntros (Hvf) "Hown He1 He2".
+    iApply (imp_wand with "[-]").
+    { iApply (imp_ERecordSet with "Hown He1 He2"). exact Hvf. }
+    iIntros (_) "(%x & HΦ & Hrecord)".
+    iExists x. iFrame "HΦ".
+    unfold ownRepr.
+    pose proof repr_id as Hid. simpl in Hid. rewrite Hid.
+    iApply "Hrecord".
+  Qed.
+
+End encoded_fields.
